\documentclass[12pt]{article}
\usepackage{amssymb}
\begin{document}
\paragraph{Part 5}
\subparagraph{Power:}
\raggedright

power $n$ $m$ := $\lambda m. \lambda n.m$ (times $n$) succ 0
\subparagraph{Pred:}
pred $n:= \lambda n$.snd.pair (succ (fst $p$)) (fst $p$) where $p := $ pair 0 0
\subparagraph{Minus:} 
minus $n$ $m := \lambda n. \lambda m.n$ pred $m$
\subparagraph{Less:}
less $n$ $m := \lambda n. \lambda m.$is-zero (minus $n$ $m$)
\subparagraph{Equal:}
equal $n$ $m := \lambda n. \lambda m$
\subparagraph{Fibbit:}
fibbit $n := \lambda n.p.$fst.pair (plus (fst $p$) (snd $p$)) fst $p$ where $p := $ pair 0 1
\subparagraph{Div2:}
div2 $n := \lambda n.$fst($n$ $t$ $p_{0}$) where $p_{0} := $pair 0 0, $t := \lambda p.$pair (snd $p$) (succ (fst $p$))
\subparagraph{Fibrec:}
fibrec $n :=$ Y (fibTemplate) $n$ where fibTemplate $n := \lambda f.\lambda n$ if (less $n$ 2) 1 f (plus (minus $n$ 2) (minus $n$ 1))
\enddocument